examples/mtac/Demo.v
@@ -12,14 +12,15 @@ Import McMtacNotation.
 
 Definition test (t : expr) : McMtacT ident (option expr) :=
   mmatch t with
-    | [ PApp (PFunc 0 nil) (PGet 0 (tvType 0)) ] =>> fun x => ret (Some x)
+    | [ PApp (PFunc 1 nil) (PGet 0 (tvType 0)) ] =>> fun x => ret (Some x)
     \ ret None
   end%mcmtac.
 
-Let tfs := {| tfenv := 0 ; tftype := tvArr (tvType 0) (tvType 0) |} ::
-           {| tfenv := 0 ; tftype := tvType 0 |} :: nil.
+Let tfs :=
+  from_tlist ({| tfenv := 0 ; tftype := tvArr (tvType 0) (tvType 0) |} ::
+              {| tfenv := 0 ; tftype := tvType 0 |} :: nil).
 Let tus : list typ := nil.
 Let tvs := (tvType 0 :: nil).
-Let exp := (App (Func 0 nil) (Var 0)).
+Let exp := (App (Func 1 nil) (Var 0)).
 
 Eval compute in unIdent (runMcMtac tfs tus tvs 10 (test exp)).
